feat: add thinning and big chamges

codes/PTS.v
@@ -1,6 +1,8 @@
 Require Import List.
 Require Import Classical.
 Import ListNotations.
+From Stdlib.Program Require Import Program Wf.
+Require Import Lia.
 
 Require Import Thesis.PTSSignature.
 
@@ -26,8 +28,8 @@ Fixpoint fv (t : term) : list var :=
     match t with
     | t_sort _   => []
     | t_var x    => [x]
-    | t_pi x A B => remove eq_var_dec x (fv A ++ fv B)
-    | t_lam x A B => remove eq_var_dec x (fv A ++ fv B)
+    | t_pi x A B => fv A ++ remove eq_var_dec x (fv B)
+    | t_lam x A B => fv A ++ remove eq_var_dec x (fv B)
     | t_app M N  => fv M ++ fv N
     end.
 
@@ -63,7 +65,7 @@ Inductive alpha_eq : term -> term -> Prop :=
   | alpha_prod_diff : forall x y A1 B1 A2 B2,
       ~ In y (fv (t_pi x A1 B1)) ->
       A1 =a A2 ->
-      B1 =a (rename x y B2) ->
+      B1 =a (rename y x B2) ->
       t_pi x A1 B1 =a t_pi y A2 B2
 
   | alpha_lam_same : forall x A1 B1 A2 B2,
@@ -74,7 +76,7 @@ Inductive alpha_eq : term -> term -> Prop :=
   | alpha_lam_diff : forall x y A1 B1 A2 B2,
       ~ In y (fv (t_lam x A1 B1)) ->
       A1 =a A2 ->
-      B1 =a (rename x y B2 ) ->
+      B1 =a (rename y x B2 ) ->
       t_lam x A1 B1 =a t_lam y A2 B2
 
 where "t1 =a t2" := (alpha_eq t1 t2).
@@ -84,35 +86,91 @@ Proof.
   induction t; constructor; auto.
 Qed.
 
-Fixpoint subst_term (x : var) (N : term) (t : term) : term :=
+Fixpoint max_var_idx (xs : list var) : nat :=
+  match xs with
+  | [] => 0
+  | v :: xs => Nat.max (var_idx v) (max_var_idx xs)
+  end.
+
+Definition fresh (s : Sort) (xs : list var) : var :=
+  mkvar s (S (max_var_idx xs)).
+
+Fixpoint size (t : term) : nat :=
+  match t with
+  | t_sort _ => 1
+  | t_var _ => 1
+  | t_app M N => 1 + size M + size N
+  | t_pi _ A B => 1 + size A + size B
+  | t_lam _ A M => 1 + size A + size M
+  end.
+
+Lemma rename_size :
+  forall x y M,
+    size (rename x y M) = size M.
+Proof.
+  intros x y M. induction M.
+    - reflexivity.
+    - simpl. destruct (eq_var_dec v x).
+      + reflexivity.
+      + reflexivity.
+    - simpl. rewrite IHM1. rewrite IHM2. reflexivity.
+    - simpl. destruct (eq_var_dec v x).
+      + simpl. rewrite IHM1. reflexivity.
+      + simpl. rewrite IHM1. rewrite IHM2. reflexivity.
+    - simpl. destruct (eq_var_dec v x).
+      + simpl. rewrite IHM1. reflexivity.
+      + simpl. rewrite IHM1. rewrite IHM2. reflexivity.
+Qed.
+
+Reserved Notation "M ⁅ x ≔ N ⁆"
+  (at level 20, left associativity).
+
+Program Fixpoint subst_term (x : var) (N : term) (t : term) {measure (size t)} : term :=
   match t with
   | t_sort s  => t_sort s
   | t_var y   => if eq_var_dec y x then N else t_var y
-  | t_app P Q => t_app (subst_term x N P) (subst_term x N Q)
+  | t_app P Q => t_app (P⁅x ≔ N⁆) (Q⁅x ≔ N⁆)
 
   | t_pi y A B =>
-      if eq_var_dec y x
-      then t_pi y (subst_term x N A) B
-      else t_pi y (subst_term x N A) (subst_term x N B)
+    let z := fresh (var_sort y) (fv N ++ fv B) in
+    t_pi z (A⁅x ≔ N⁆) ((rename y z B)⁅x ≔ N⁆)
 
   | t_lam y A M =>
-      if eq_var_dec y x
-      then t_lam y (subst_term x N A) M
-      else t_lam y (subst_term x N A) (subst_term x N M)
-  end. 
-
+    let z := fresh (var_sort y) (fv N ++ fv M) in
+    t_lam z (A⁅x ≔ N⁆) ((rename y z M)⁅x ≔ N⁆)
+  end
+  
+where "M ⁅ x ≔ N ⁆" := (subst_term x N M).
+Next Obligation.
+  simpl. lia.
+Qed.
+Next Obligation.
+  simpl. lia.
+Qed.
+Next Obligation.
+  simpl. lia.
+Qed.
+Next Obligation.
+  rewrite rename_size. simpl. lia.
+Qed.
+Next Obligation.
+  simpl. lia.
+Qed.
+Next Obligation.
+  rewrite rename_size. simpl. lia.
+Qed.
 
 Definition beta (M N : term) : Prop :=
   exists x A Body Arg,
     M = t_app (t_lam x A Body) Arg /\
-    N = subst_term x Arg Body.
+    N = Body⁅x ≔ Arg⁆.
 
 Reserved Notation "M ->b N" (at level 70, no associativity).
 
 Inductive beta_red : term -> term -> Prop :=
 
   | beta_base : forall x A M N,
-      t_app (t_lam x A M) N ->b subst_term x N M
+      t_app (t_lam x A M) N ->b M⁅x ≔ N⁆
 
   | beta_app_l : forall M M' N,
       M ->b M' ->
@@ -271,44 +329,34 @@ Fixpoint lookup (c : context) (x : var) : option term :=
       else lookup c' x
   end.
 
-Definition in_ctx (x : var) (c : context) : Prop :=
-  exists A, lookup c x = Some A.
+Definition dom (Γ : context) : list var :=
+  map fst Γ.
 
-Definition is_fresh (x : var) (c : context) : Prop :=
-  lookup c x = None.
-
-Fixpoint dom (c : context) : list var :=
-  match c with
-  | [] => []
-  | (x, _) :: c' => x :: dom c'
-  end.
-
+Definition is_fresh (x : var) (Γ : context) :=
+  ~ In x (dom Γ).
 
 Reserved Notation "Γ ⊢ M ∈ A" (at level 70, no associativity).
 
 Inductive typing : context -> term -> term -> Prop :=
-  | typing_axiom : forall Γ s s',
+  | typing_axiom : forall s s',
       A s s' ->
-      Γ ⊢ (t_sort s) ∈ (t_sort s')
+      [] ⊢ t_sort s ∈ t_sort s'
 
-  | typing_var : forall Γ x A s,
+  | typing_var : forall Γ x A,
       is_fresh x Γ ->
-      var_sort x = s ->
-      Γ ⊢ A ∈ t_sort s ->
+      Γ ⊢ A ∈ t_sort (var_sort x) ->
       Γ ++ [(x, A)] ⊢ t_var x ∈ A
 
-  | typing_weak : forall Γ x B M A s,
+  | typing_weak : forall Γ x B M A,
       is_fresh x Γ ->
-      var_sort x = s ->
       Γ ⊢ M ∈ A ->
-      Γ ⊢ B ∈ t_sort s ->
+      Γ ⊢ B ∈ t_sort (var_sort x) ->
       Γ ++ [(x, B)] ⊢ M ∈ A
 
-  | typing_pi : forall Γ x A B s1 s2 s',
-      var_sort x = s1 ->
-      Γ ⊢ A ∈ t_sort s1 ->
-      Γ ++ [(x, A)] ⊢ B ∈ t_sort s2 ->
-      R s1 s2 s' ->
+  | typing_pi : forall Γ x A B s s',
+      Γ ⊢ A ∈ t_sort (var_sort x) ->
+      Γ ++ [(x, A)] ⊢ B ∈ t_sort s ->
+      R (var_sort x) s s' ->
       Γ ⊢ (t_pi x A B) ∈ (t_sort s')
 
   | typing_lam : forall Γ x A M B s',
@@ -319,7 +367,7 @@ Inductive typing : context -> term -> term -> Prop :=
   | typing_app : forall Γ M N A B x,
       Γ ⊢ M ∈ t_pi x A B ->
       Γ ⊢ N ∈ A ->
-      Γ ⊢ t_app M N ∈ (subst_term x N B)
+      Γ ⊢ t_app M N ∈ (B⁅x ≔ N⁆)
 
   | typing_conv : forall Γ M A B s,
       Γ ⊢ M ∈ A ->
@@ -328,6 +376,191 @@ Inductive typing : context -> term -> term -> Prop :=
       Γ ⊢ M ∈ B
 
 where "Γ ⊢ M ∈ A" := (typing Γ M A).
+
+Definition legal (Γ : context) : Prop :=
+  exists M N, Γ ⊢ M ∈ N.
+
+(* Meta-Theory *)
+
+Lemma start_axiom :
+  forall Γ s s',
+    legal Γ ->
+    A s s' ->
+    Γ ⊢ t_sort s ∈ t_sort s'.
+Proof.
+  intros Γ s s' Hl Hs. destruct Hl as [M [N Htyp]].
+  induction Htyp; auto.
+  - apply typing_axiom. apply Hs.
+  - apply typing_weak.
+    + apply H.
+    + apply IHHtyp.
+    + apply Htyp.
+  - apply typing_weak.
+    + apply H.
+    + apply IHHtyp1.
+    + apply Htyp2.
+Qed.
+
+Lemma start_var :
+  forall Γ x T,
+    legal Γ ->
+    In (x,T) Γ ->
+    Γ ⊢ t_var x ∈ T.
+Proof.
+  intros Γ x T Hl Hin. destruct Hl as [M [N Htyp]].
+  induction Htyp; auto.
+
+  - contradiction.
+
+  - apply in_app_or in Hin. destruct Hin as [Hin | Hin].
+    + apply typing_weak.
+      * apply H.
+      * apply IHHtyp. apply Hin.
+      * apply Htyp.
+    + destruct Hin as [Hin | []]. inversion Hin. subst. apply typing_var.
+      * apply H.
+      * apply Htyp.
+  
+  - apply in_app_or in Hin. destruct Hin as [Hin | Hin].
+    + apply typing_weak.
+      * apply H.
+      * apply IHHtyp1. apply Hin.
+      * apply Htyp2.
+    + destruct Hin as [Hin | []]. inversion Hin. subst. apply typing_var.
+      * apply H.
+      * apply Htyp2.
+Qed.
+
+Definition subcontext (Γ Δ : context) : Prop :=
+  forall x T,
+    In (x, T) Γ ->
+    In (x, T) Δ.
+
+Notation "Γ ⊆ Δ" := (subcontext Γ Δ) (at level 70, no associativity).
+
+Lemma subcontext_extend : forall Γ Δ z A,
+  Γ ⊆ Δ ->
+  is_fresh z Δ ->
+  Γ ++ [(z, A)] ⊆ Δ ++ [(z, A)].
+Proof.
+  intros Γ Δ z A Hsub Hfr y T Hin.
+  apply in_app_or in Hin.
+  destruct Hin.
+  - apply in_or_app. left. apply Hsub. assumption.
+  - simpl in H.
+    destruct H as [H | H].
+    + inversion H; subst.
+      apply in_or_app. right. left. reflexivity.
+    + contradiction.
+Qed.
+
+Lemma subcontext_extend_r : forall Γ x T, Γ ⊆ Γ ++ [(x, T)].
+Proof.
+  intros.
+  unfold subcontext. intros.
+  apply in_or_app. left.
+  apply H.
+Qed.
+
+Axiom thinning_fresh : forall Γ Δ x T M N,
+  legal Δ ->
+  Γ ⊆ Δ ->
+  Γ ++ [(x, T)] ⊢ M ∈ N ->
+  is_fresh x Δ.
+
+Axiom pi_domain_valid : forall Γ x A B s',
+  Γ ⊢ t_pi x A B ∈ t_sort s' ->
+  Γ ⊢ A ∈ t_sort (var_sort x).
+
+Lemma thinning :
+  forall Γ Δ M N,
+    legal Δ ->
+    Γ ⊆ Δ ->
+    Γ ⊢ M ∈ N ->
+    Δ ⊢ M ∈ N.
+Proof.
+  intros Γ Δ M N Hleg Hsub Htyp.
+  generalize dependent Δ.
+  induction Htyp; intros Δ Hleg Hsub.
+
+  - apply start_axiom.
+    + apply Hleg.
+    + apply H.
+
+  - apply start_var.
+    + apply Hleg.
+    + unfold subcontext in Hsub. apply Hsub. apply in_or_app. right. 
+    simpl. left. reflexivity.
+  
+  - apply IHHtyp1. 
+    + apply Hleg.
+    + unfold subcontext in Hsub. unfold subcontext. intros y T Hin. 
+    apply Hsub. apply in_or_app. left. apply Hin.
+
+  - apply typing_pi with s.
+    + apply IHHtyp1.
+      * apply Hleg.
+      * apply Hsub.
+    + apply IHHtyp2.
+      * exists (t_var x). exists (A0). apply typing_var.
+        ** apply thinning_fresh with (Γ:=Γ) (x:=x) (T:=A0) (M:=B) (N:=t_sort s); auto.
+        ** apply IHHtyp1.
+          *** apply Hleg.
+          *** apply Hsub.
+      * apply subcontext_extend.
+        ** apply Hsub.
+        ** apply thinning_fresh with (Γ:=Γ) (x:=x) (T:=A0) (M:=B) (N:=t_sort s); auto.
+    + apply H.
+
+  - apply typing_lam with s'.
+    + apply IHHtyp1.
+      * exists (t_var x). exists (A0). apply typing_var.
+        ** apply thinning_fresh with (Γ:=Γ) (x:=x) (T:=A0) (M:=M) (N:=B); auto.
+        ** apply pi_domain_valid with (B:=B) (s':=s'). apply IHHtyp2; auto.
+      * apply subcontext_extend.
+        ** apply Hsub.
+        ** apply thinning_fresh with (Γ:=Γ) (x:=x) (T:=A0) (M:=M) (N:=B); auto.
+    + apply IHHtyp2.
+      * apply Hleg.
+      * apply Hsub.
+
+  - apply typing_app with A0; auto.
+
+  - apply typing_conv with A0 s; auto. 
+Qed.
+
+Lemma app_singleton_injective :
+  forall (Γ Δ : context)
+         (x y : var)
+         (M N : term),
+    Γ ++ [(x, M)] = Δ ++ [(y, N)] ->
+    Γ = Δ /\ x = y /\ M = N.
+Proof.
+  induction Γ as [| [v T] Γ IH].
+  - intros Δ x y M N H.
+    destruct Δ as [| [v' T'] Δ].
+    + simpl in H.
+      inversion H. subst.
+      repeat split; reflexivity.
+    + simpl in H.
+      destruct Δ.
+      * discriminate.
+      * discriminate.
+
+  - intros Δ x y M N H.
+    destruct Δ as [| [v' T'] Δ].
+    + simpl in H.
+      destruct Γ.
+      * discriminate.
+      * discriminate.
+
+    + simpl in H.
+      inversion H. subst.
+      specialize (IH Δ x y M N H3).
+      destruct IH as [HΓ [Hx HM]].
+      subst.
+      repeat split; reflexivity.
+Qed.
 
 Lemma generation_sort :
   forall Γ s W,
@@ -357,8 +590,8 @@ Proof.
     + reflexivity.
     + contradiction.
   - destruct a as (v, T). simpl in *. destruct (eq_var_dec y v) as [Heq | Hneq].
-    + discriminate F.
-    + apply IHC. apply F.
+    + unfold not in F. destruct F. left. symmetry. apply Heq.
+    + apply IHC. unfold not. intros. unfold not in F. apply F. right. apply H.
 Qed.
 
 Lemma lookup_extend :
@@ -383,33 +616,50 @@ Proof.
   remember (t_var x) as T.
   induction H; inversion HeqT; subst.
 
-  - exists A0. split.
-    + apply lookup_fresh. apply H.
-    + split.
-      * apply typing_weak with (s := var_sort x).
-        ** apply H.
-        ** reflexivity.
-        ** apply H1.
-        ** apply H1.
-      * apply beq_refl.
+  - exists A0. repeat split; auto.
+    + apply lookup_fresh; auto.
+    + apply typing_weak; auto.
+    + apply beq_refl.
   
-  - apply IHtyping1 in H3. destruct H3 as [B' [Q1 [Q2 Q3]]]. exists B'. split.
-    + apply lookup_extend. apply Q1.
-    + split.
-      * apply typing_weak with (x := x0) (B := B) (s := var_sort x0).
-        ** apply H.
-        ** reflexivity.
-        ** apply Q2.
-        ** apply H2.
-      * apply Q3.
-
-  - apply IHtyping1 in H2. destruct H2 as [B' [Q1 [Q2 Q3]]]. exists B'. split.
-    + apply Q1.
-    + split.
-      * apply Q2.
-      * apply beq_trans with A0.
-        ** apply beq_sym. apply H0.
-        ** apply Q3.
+  - apply IHtyping1 in H2. destruct H2 as [B' [Q1 [Q2 Q3]]]. exists B'. repeat split; auto.
+    + apply lookup_extend; auto.
+    + apply typing_weak; auto.
+    
+  - apply IHtyping1 in H2. destruct H2 as [B' [Q1 [Q2 Q3]]]. exists B'. repeat split; auto.
+    apply beq_trans with A0; auto. apply beq_sym; auto.
 Qed.
+
+Lemma generation_pi : 
+  forall Γ x B C W, 
+    Γ ⊢ t_pi x B C ∈ W ->
+    exists s' s'',
+      Γ ⊢ B ∈ t_sort (var_sort x) /\
+      (Γ ++ [(x,B)]) ⊢ C ∈ t_sort s' /\
+      Sig.R (var_sort x) s' s'' /\
+      W =b t_sort s''.
+Proof.
+  intros Γ x B C W H. 
+  remember (t_pi x B C) as T eqn:HT.
+  induction H; inversion HT; subst.
+
+  - apply IHtyping1 in H2. destruct H2 as [s' [s'' [HB [HC [HR Heq]]]]].
+  exists s'. exists s''. repeat split; auto.
+    + apply typing_weak; auto.
+    + apply thinning with (Γ ++ [(x, B)]).
+      * exists (t_var x). exists B. apply typing_var.
+        ** apply thinning_fresh with (Γ:=Γ) (T:=B) (M:=C) (N:=t_sort s'); auto.
+          *** exists (t_var x0). exists (B0). apply typing_var; auto.
+          *** apply subcontext_extend_r.
+        ** apply thinning with Γ; auto.
+          *** exists (t_var x0). exists (B0). apply typing_var; auto.
+          *** apply subcontext_extend_r.
+      * apply subcontext_extend.
+        ** apply subcontext_extend_r.
+        ** apply thinning_fresh with (Γ:=Γ) (T:=B) (M:=C) (N:=t_sort s'); auto.
+          *** exists (t_var x0). exists (B0). apply typing_var; auto.
+          *** apply subcontext_extend_r.
+      * apply HC.
+  
+  -
 
 End PTS.
